Phi_Examples/Quicksort.thy
@@ -5,58 +5,71 @@ theory Quicksort
 begin
 
 declare [[auto_sledgehammer_params = "try0 = false"]]
-proc qsort:
-  input  \<open>i \<Ztypecolon> \<v>\<a>\<l> \<bbbS>\<p>\<t>\<r>[addr:LEN] \<i>\<n>\<t>\<heavy_comma> \<comment> \<open>\<open>LEN\<close> is the length of the entire array, which decides
-                                            the scope that a slice pointer can range over.\<close>
-          len \<Ztypecolon> \<v>\<a>\<l> \<nat>(\<i>\<n>\<t>)\<heavy_comma>
-          l \<Ztypecolon> \<m>\<e>\<m>[addr] \<s>\<l>\<i>\<c>\<e>[i,len] \<nat>(\<i>\<n>\<t>)\<close>
-  premises \<open>i + len \<le> LEN\<close>
-  output \<open>l' \<Ztypecolon> \<m>\<e>\<m>[addr] \<s>\<l>\<i>\<c>\<e>[i,len] \<nat>(\<i>\<n>\<t>) \<s>\<u>\<b>\<j> l'. l <~~> l' \<and> sorted l'\<close>
-  is [recursive]
-  is [routine]
-\<medium_left_bracket>
-  if (len \<le> 1)
-  \<medium_left_bracket> return \<medium_right_bracket>
-  \<medium_left_bracket>
-    val pivot \<leftarrow> *(i + (len - 1)) \<semicolon>
-    var d \<leftarrow> 0 \<semicolon>
-    iterate (0,len) \<open>\<lambda>n. d \<Ztypecolon> \<v>\<a>\<r>[d] \<nat>(\<i>\<n>\<t>)\<heavy_comma>
-                          l' \<Ztypecolon> \<m>\<e>\<m>[addr] \<s>\<l>\<i>\<c>\<e>[i,len] \<nat>(\<i>\<n>\<t>)
-                         \<s>\<u>\<b>\<j> l' d.
-                           d \<le> n \<and> l <~~> l' \<and>
-                           (\<forall>k<d. l' ! k \<le> ?pivot) \<and>
-                           (\<forall>k<n-d. ?pivot < l' ! (d + k)) \<close> 
-    \<medium_left_bracket> 
-      for n \<rightarrow> val n \<semicolon>
-      *(i + n) \<rightarrow> val x \<semicolon>
-      if (x \<le> pivot)
-      \<medium_left_bracket>
-        (i + n) := *(i + d) \<semicolon>
-        (i + d) := x \<semicolon>
-        d \<leftarrow> d + 1
-      \<medium_right_bracket>
-      \<medium_left_bracket> \<medium_right_bracket> \<semicolon>
-    \<medium_right_bracket>
-    qsort (i, d) \<semicolon>
-    qsort (i + d, len - d) \<semicolon>
-        
-    holds_fact t1: \<open>(\<forall>x\<in>set (drop d l'). l ! (len - 1) < x)\<close>
-           and t2: \<open>(\<forall>x\<in>set (take d l'). x \<le> l ! (len - 1))\<close>
-           and t4[\<phi>sledgehammer_simps]: \<open>set l'b = set (drop d l')\<close>
-    from \<open>mset (take d l') = mset l'a\<close> have t3[\<phi>sledgehammer_simps]: \<open>set l'a = set (take d l')\<close> by auto_sledgehammer
-    note [\<phi>sledgehammer_simps] = sorted_append  \<semicolon>
 
-    return
-  \<medium_right_bracket>
-\<medium_right_bracket> .
+
+
+  proc qsort:
+    input  \<open>\<v>\<a>\<l> i \<Ztypecolon> \<s>\<l>\<i>\<c>\<e>\<bbbP>\<t>\<r>[addr:LEN] \<i>\<n>\<t>\<heavy_comma>
+            \<v>\<a>\<l> len \<Ztypecolon> \<nat>(\<i>\<n>\<t>)\<heavy_comma>
+            l \<Ztypecolon> \<m>\<e>\<m>[addr] \<s>\<l>\<i>\<c>\<e>[i,len] \<nat>(\<i>\<n>\<t>)\<close>
+    premises \<open>i + len \<le> LEN\<close>
+    output \<open>l' \<Ztypecolon> \<m>\<e>\<m>[addr] \<s>\<l>\<i>\<c>\<e>[i,len] \<nat>(\<i>\<n>\<t>)
+            \<s>\<u>\<b>\<j> l'. l <~~> l' \<and> sorted l'\<close>
+    is [recursive]
+    is [routine]
+  \<medium_left_bracket>
+    if (len \<le> 1) \<medium_left_bracket>
+      return
+    \<medium_right_bracket> \<medium_left_bracket>
+      val pivot \<leftarrow> *(i + (len - 1)) \<semicolon>
+      var d \<leftarrow> 0 \<semicolon>
+      iterate (0,len) \<open>\<lambda>n. d  \<Ztypecolon> \<v>\<a>\<r>[d] \<nat>(\<i>\<n>\<t>)\<heavy_comma>
+                           l' \<Ztypecolon> \<m>\<e>\<m>[addr] \<s>\<l>\<i>\<c>\<e>[i,len] \<nat>(\<i>\<n>\<t>)
+                           \<s>\<u>\<b>\<j> l' d.
+                             d \<le> n \<and> l <~~> l' \<and>
+                             (\<forall>k<d. l' ! k \<le> ?pivot) \<and>
+                             (\<forall>k<n-d. ?pivot < l' ! (d + k)) \<close> 
+      \<medium_left_bracket>
+        for n \<rightarrow> val n \<semicolon>
+        *(i + n) \<rightarrow> val x \<semicolon>
+        if (x \<le> pivot) \<medium_left_bracket>
+          (i + n) := *(i + d) \<semicolon>
+          (i + d) := x \<semicolon>
+          d \<leftarrow> d + 1
+        \<medium_right_bracket> \<medium_left_bracket>
+          (*comment: else, do nothing*)
+        \<medium_right_bracket> \<semicolon>
+      \<medium_right_bracket>
+      qsort (i, d) \<semicolon>
+      qsort (i + d, len - d) \<semicolon>
+          
+      holds_fact t1: \<open>(\<forall>x\<in>set (drop d l'). l ! (len - 1) < x)\<close>
+             and t2: \<open>(\<forall>x\<in>set (take d l'). x \<le> l ! (len - 1))\<close>
+             and t3[simp]: \<open>set l'b = set (drop d l')\<close>
+             and t4[simp]: \<open>set l'a = set (take d l')\<close> \<semicolon>
+  
+      return
+    \<medium_right_bracket>
+  \<medium_right_bracket> .
 
 
 text \<open>The Conclusions of above Certification is the following Specification Theorems\<close>
 
 thm qsort_\<phi>app
 
+context 
+  fixes i len LEN :: nat
+    and \<a>\<r>\<g>1 \<a>\<r>\<g>2 :: \<open>VAL \<phi>arg\<close>
+    and addr :: \<open>VAL aggregate_index' list memaddr\<close>
+    and l :: \<open>nat list\<close>
+begin
+
+thm qsort_\<phi>app[of i len LEN \<a>\<r>\<g>1 \<a>\<r>\<g>2 addr l]
+
+end
+
 text \<open>Semantic Representations of the Programs: \<close>
- 
+  
 thm qsort_def
 
 end
