Phi_Semantics/PhiSem_Mem_C_Ar_AI.thy
@@ -5,25 +5,25 @@ begin
 section \<open>Pointer Arithmetic\<close>
 
 proc op_add_ptr_a[\<phi>overload +]:
-  input  \<open>i \<Ztypecolon> \<v>\<a>\<l> \<bbbS>\<p>\<t>\<r>[addr:len] TY\<heavy_comma> j \<Ztypecolon> \<v>\<a>\<l> \<int>\<close>
+  input  \<open>i \<Ztypecolon> \<v>\<a>\<l> \<s>\<l>\<i>\<c>\<e>\<bbbP>\<t>\<r>[addr:len] TY\<heavy_comma> j \<Ztypecolon> \<v>\<a>\<l> \<int>\<close>
   premises \<open>0 \<le> int i + j \<and> nat (int i + j) \<le> len\<close>
-  output \<open>nat (int i + j) \<Ztypecolon> \<v>\<a>\<l> \<bbbS>\<p>\<t>\<r>[addr:len] TY\<close>
+  output \<open>nat (int i + j) \<Ztypecolon> \<v>\<a>\<l> \<s>\<l>\<i>\<c>\<e>\<bbbP>\<t>\<r>[addr:len] TY\<close>
 \<medium_left_bracket>
   $i semantic_local_value \<p>\<t>\<r>
   $j semantic_local_value \<a>\<i>\<n>\<t>
 
   semantic_return \<open>
       sem_mk_pointer (sem_dest_pointer (\<phi>arg.dest \<a>\<r>\<g>1) ||+ of_int (sem_dest_aint (\<phi>arg.dest \<a>\<r>\<g>2)) * of_nat (MemObj_Size TY))
-          \<Turnstile> (nat (int i + j) \<Ztypecolon> \<bbbS>\<p>\<t>\<r>[addr:len] TY)\<close>
+          \<Turnstile> (nat (int i + j) \<Ztypecolon> \<s>\<l>\<i>\<c>\<e>\<bbbP>\<t>\<r>[addr:len] TY)\<close>
     certified by (clarsimp simp: address_to_raw_array_GEP[OF \<open>address_type addr = \<a>\<r>\<r>\<a>\<y>[len] TY\<close>] useful distrib_right,
                   simp add: add.commute)
 
 \<medium_right_bracket> .
 
 proc (nodef) op_add_ptr_aN[\<phi>overload +]:
-  input  \<open>i \<Ztypecolon> \<v>\<a>\<l> \<bbbS>\<p>\<t>\<r>[addr:len] TY\<heavy_comma> j \<Ztypecolon> \<v>\<a>\<l> \<nat>\<close>
+  input  \<open>i \<Ztypecolon> \<v>\<a>\<l> \<s>\<l>\<i>\<c>\<e>\<bbbP>\<t>\<r>[addr:len] TY\<heavy_comma> j \<Ztypecolon> \<v>\<a>\<l> \<nat>\<close>
   premises \<open>i + j \<le> len\<close>
-  output \<open>i + j \<Ztypecolon> \<v>\<a>\<l> \<bbbS>\<p>\<t>\<r>[addr:len] TY\<close>
+  output \<open>i + j \<Ztypecolon> \<v>\<a>\<l> \<s>\<l>\<i>\<c>\<e>\<bbbP>\<t>\<r>[addr:len] TY\<close>
 \<medium_left_bracket>
   $i + $j
 \<medium_right_bracket> .
