Phi_Semantics/PhiSem_Mem_C_Ar_MI.thy
@@ -5,9 +5,9 @@ begin
 section \<open>Pointer Arithmetic\<close>
 
 proc op_add_ptr[\<phi>overload +]:
-  input  \<open>i \<Ztypecolon> \<v>\<a>\<l> \<bbbS>\<p>\<t>\<r>[addr:len] TY\<heavy_comma> j \<Ztypecolon> \<v>\<a>\<l> \<int>('b)\<close>
+  input  \<open>i \<Ztypecolon> \<v>\<a>\<l> \<s>\<l>\<i>\<c>\<e>\<bbbP>\<t>\<r>[addr:len] TY\<heavy_comma> j \<Ztypecolon> \<v>\<a>\<l> \<int>('b)\<close>
   premises \<open>0 \<le> int i + j \<and> nat (int i + j) \<le> len\<close>
-  output \<open>nat (int i + j) \<Ztypecolon> \<v>\<a>\<l> \<bbbS>\<p>\<t>\<r>[addr:len] TY\<close>
+  output \<open>nat (int i + j) \<Ztypecolon> \<v>\<a>\<l> \<s>\<l>\<i>\<c>\<e>\<bbbP>\<t>\<r>[addr:len] TY\<close>
 \<medium_left_bracket>
   $i semantic_local_value \<p>\<t>\<r>
   $j semantic_local_value \<open>\<i>\<n>\<t>('b)\<close> 
@@ -18,16 +18,16 @@ proc op_add_ptr[\<phi>overload +]:
   semantic_return \<open>
       sem_mk_pointer (sem_dest_pointer (\<phi>arg.dest \<a>\<r>\<g>1)
               ||+ Word.scast (of_nat (snd (sem_dest_int (\<phi>arg.dest \<a>\<r>\<g>2))) :: 'b word) * of_nat (MemObj_Size TY))
-          \<Turnstile> (nat (int i + j) \<Ztypecolon> \<bbbS>\<p>\<t>\<r>[addr:len] TY)\<close>
+          \<Turnstile> (nat (int i + j) \<Ztypecolon> \<s>\<l>\<i>\<c>\<e>\<bbbP>\<t>\<r>[addr:len] TY)\<close>
   certified by (insert useful, auto simp: address_to_raw_array_GEP[OF \<open>address_type addr = \<a>\<r>\<r>\<a>\<y>[len] TY\<close>] distrib_right,
                 simp add: add.commute signed_of_int signed_take_bit_int_eq_self)
 \<medium_right_bracket> .
 
 
 proc op_add_ptr_unsigned[\<phi>overload +]:
-  input  \<open>i \<Ztypecolon> \<v>\<a>\<l> \<bbbS>\<p>\<t>\<r>[addr:len] TY\<heavy_comma> j \<Ztypecolon> \<v>\<a>\<l> \<nat>('b)\<close>
+  input  \<open>i \<Ztypecolon> \<v>\<a>\<l> \<s>\<l>\<i>\<c>\<e>\<bbbP>\<t>\<r>[addr:len] TY\<heavy_comma> j \<Ztypecolon> \<v>\<a>\<l> \<nat>('b)\<close>
   premises \<open>i + j \<le> len\<close>
-  output \<open>i + j \<Ztypecolon> \<v>\<a>\<l> \<bbbS>\<p>\<t>\<r>[addr:len] TY\<close>
+  output \<open>i + j \<Ztypecolon> \<v>\<a>\<l> \<s>\<l>\<i>\<c>\<e>\<bbbP>\<t>\<r>[addr:len] TY\<close>
 \<medium_left_bracket>
   $i semantic_local_value \<p>\<t>\<r>
   $j semantic_local_value \<open>\<i>\<n>\<t>('b)\<close>
@@ -35,7 +35,7 @@ proc op_add_ptr_unsigned[\<phi>overload +]:
   semantic_return \<open>
       sem_mk_pointer (sem_dest_pointer (\<phi>arg.dest \<a>\<r>\<g>1)
               ||+ Word.ucast (of_nat (snd (sem_dest_int (\<phi>arg.dest \<a>\<r>\<g>2))) :: 'b word) * of_nat (MemObj_Size TY))
-          \<Turnstile> (i + j \<Ztypecolon> \<bbbS>\<p>\<t>\<r>[addr:len] TY)\<close>
+          \<Turnstile> (i + j \<Ztypecolon> \<s>\<l>\<i>\<c>\<e>\<bbbP>\<t>\<r>[addr:len] TY)\<close>
   certified by (insert useful,
                 auto simp: address_to_raw_array_GEP[OF \<open>address_type addr = \<a>\<r>\<r>\<a>\<y>[len] TY\<close>]
                            distrib_right ucast_of_nat_small, simp add: add.commute)
